Rollback lrefs (sad noises)

state/TargetLangIFC.fst
@@ -7,101 +7,6 @@ open FStar.Tactics.Typeclasses
 open Monotonic.IFC.Heap
 open IFC.Heap.ST
 
-(** target_lang is a shallow embedding of STLC **)
-class target_lang (t:Type) = {
-  deep_contains : lheap -> t -> Type0;
-  deeply_labeled_with_low : t -> lheap -> Type0; (** deep check that the object points to low things **)
-
-  deep_recall : (r:t) -> ST unit 
-              (requires (fun h -> True))
-              (ensures  (fun h0 _ h1 -> h0 == h1 /\ h1 `deep_contains` r /\ deeply_labeled_with_low r h1));  
-}
-  
-instance target_lang_unit : target_lang unit = {
-  deep_contains = (fun _ _ -> True);
-  deep_recall = (fun _ -> ());
-
-  deeply_labeled_with_low = (fun _ _ -> True);
-}
-
-instance target_lang_int : target_lang int = {
-  deep_contains = (fun _ _ -> True);
-  deep_recall = (fun _ -> ());
-
-  deeply_labeled_with_low = (fun _ _ -> True);
-}
-
-instance target_lang_pair (t1:Type) (t2:Type) {| c1:target_lang t1 |} {| c2:target_lang t2 |} : target_lang (t1 * t2) = {
-  deep_contains = (fun h (x1, x2) -> h `deep_contains` x1 /\ h `deep_contains` x2);
-  deep_recall = (fun (x1, x2) -> c1.deep_recall x1; c2.deep_recall x2);
-
-  deeply_labeled_with_low = (fun (x1, x2) h -> c1.deeply_labeled_with_low x1 h /\ c2.deeply_labeled_with_low x2 h);
-}
-
-instance target_lang_sum (t1:Type) (t2:Type) {| c1:target_lang t1 |} {| c2:target_lang t2 |} : target_lang (either t1 t2) = {
-  deep_contains = (fun h x ->
-    match x with
-    | Inl x1 -> h `deep_contains` x1
-    | Inr x2 -> h `deep_contains` x2);
-  deep_recall = (fun x ->
-    match x with
-    | Inl x1 -> c1.deep_recall x1
-    | Inr x2 -> c2.deep_recall x2);
-
-  deeply_labeled_with_low = (fun x h ->
-    match x with
-    | Inl x1 -> c1.deeply_labeled_with_low x1 h
-    | Inr x2 -> c2.deeply_labeled_with_low x2 h);
-}
-
-instance target_lang_ref (t:Type) {| c:target_lang t |} : target_lang (lref t) = {
-  deep_contains = (fun h (x:lref t) -> h `contains` x /\ h `deep_contains` (sel h x));
-
-  deeply_labeled_with_low = (fun (x:lref t) h -> label_of x h == Low /\ c.deeply_labeled_with_low (sel h x) h);  
-  deep_recall = (fun (x:lref t) -> 
-    recall x; 
-    gst_recall (is_low_pred x);
-    c.deep_recall !x);
-}
-
-open FStar.Preorder
-
-unfold let pre_tgt_arrow
-  (#t1:Type) (x:t1) {| tgtx:target_lang t1 |}
-  (h0:lheap) =
-  h0 `deep_contains` x /\                                                (* required to instantiate the properties of modifies *)
-  deeply_labeled_with_low x h0                                           (* x is Low *)
-
-let post_tgt_arrow
-  (#t1:Type) (x:t1) {| tgtx:target_lang t1 |}
-  (#t2:t1 -> Type) {| tgtr : (x:t1 -> target_lang (t2 x)) |}
-  (h0:lheap) (r:t2 x) (h1:lheap) =
-  modifies_only_label Low h0 h1 /\                                       (* allows low references to be modified *)
-  modifies_classification Set.empty h0 h1 /\                             (* no modifications of the classification *)
-
-  (h1 `(tgtr x).deep_contains` r) /\
-  ((tgtr x).deeply_labeled_with_low r h1)                                (* r is deeply labeled with Low *)
-
-let mk_tgt_arrow 
-  (t1:Type)
-  {| tgt_t1: target_lang t1 |}
-  (t2:t1 -> Type) (* TODO: this dependency is not needed anymore *)
-  {| c2 : (x:t1 -> target_lang (t2 x)) |}
-= x:t1 -> ST (t2 x) 
-    (requires (pre_tgt_arrow x #tgt_t1))
-    (ensures (post_tgt_arrow x #tgt_t1 #t2 #c2))
-
-instance target_lang_arrow 
-  (t1:Type)
-  {| target_lang t1 |}
-  (t2:t1 -> Type)
-  {| (x:t1 -> target_lang (t2 x)) |}
-  : target_lang (mk_tgt_arrow t1 t2) = {
-    deep_contains = (fun _ _ -> True);
-    deep_recall = (fun _ -> ());
-
-    deeply_labeled_with_low = (fun _ _ -> True);
-  }
 
 let prog () =
   let r : ref int = alloc 0 in
@@ -114,6 +19,90 @@ let prog () =
   let r1 : ref int = alloc 0 in
   declassify r1 Medium;
   ()
+
+(** target_lang is a shallow embedding of STLC **)
+class target_lang (t:Type) = {
+  witnessed_with_low : t -> Type0;
+}
+  
+instance target_lang_unit : target_lang unit = {
+  witnessed_with_low = (fun _ -> True);
+}
+
+instance target_lang_int : target_lang int = {
+  witnessed_with_low = (fun _ -> True);
+}
+
+instance target_lang_pair (t1:Type) (t2:Type) {| c1:target_lang t1 |} {| c2:target_lang t2 |} : target_lang (t1 * t2) = {
+  witnessed_with_low = (fun (x1, x2) -> c1.witnessed_with_low x1 /\ c2.witnessed_with_low x2);
+}
+
+instance target_lang_sum (t1:Type) (t2:Type) {| c1:target_lang t1 |} {| c2:target_lang t2 |} : target_lang (either t1 t2) = {
+  witnessed_with_low = (fun x ->
+    match x with
+    | Inl x1 -> c1.witnessed_with_low x1
+    | Inr x2 -> c2.witnessed_with_low x2);
+}
+
+instance target_lang_ref (t:Type) {| c:target_lang t |} : target_lang (ref t) = {
+  witnessed_with_low = (fun (x:ref t) -> witnessed (is_low_pred x));
+}
+
+open FStar.Preorder
+
+let inv_low_points_to_low (h:lheap) =
+  forall (a:Type) (c:target_lang a) (r:ref a). witnessed (is_low_pred r) ==>
+    c.witnessed_with_low (sel h r)
+
+effect IST (a:Type) (pre:st_pre) (post: (h:lheap -> Tot (st_post' a (pre h)))) =
+  ST a 
+    (requires (fun h0 -> 
+      inv_low_points_to_low h0 /\
+      pre h0))
+    (ensures (fun h0 r h1 ->
+      inv_low_points_to_low h1 /\
+      post h0 r h1))
+
+let alloc (#a:Type) (#rel:preorder a) (init:a)
+: IST (mref a rel) (fun h -> True) (alloc_post #a #rel init)
+=
+  let r = alloc init in
+  let h1 = get () in
+  assume (inv_low_points_to_low h1);
+  r
+
+unfold let pre_tgt_arrow
+  (#t1:Type) (x:t1) {| tgtx:target_lang t1 |}
+  (h0:lheap) =
+  witnessed_with_low x                                           (* x is Low *)
+
+let post_tgt_arrow
+  (#t1:Type) (x:t1) {| tgtx:target_lang t1 |}
+  (#t2:t1 -> Type) {| tgtr : (x:t1 -> target_lang (t2 x)) |}
+  (h0:lheap) (r:t2 x) (h1:lheap) =
+  modifies_only_label Low h0 h1 /\                                       (* allows low references to be modified *)
+  modifies_classification Set.empty h0 h1 /\                             (* no modifications of the classification *)
+
+  ((tgtr x).witnessed_with_low r)                                (* r is deeply labeled with Low *)
+
+let mk_tgt_arrow 
+  (t1:Type)
+  {| tgt_t1: target_lang t1 |}
+  (t2:t1 -> Type) (* TODO: this dependency is not needed anymore *)
+  {| c2 : (x:t1 -> target_lang (t2 x)) |}
+= x:t1 -> IST (t2 x) 
+    (requires (pre_tgt_arrow x #tgt_t1))
+    (ensures (post_tgt_arrow x #tgt_t1 #t2 #c2))
+
+instance target_lang_arrow 
+  (t1:Type)
+  {| target_lang t1 |}
+  (t2:t1 -> Type)
+  {| (x:t1 -> target_lang (t2 x)) |}
+  : target_lang (mk_tgt_arrow t1 t2) = {
+    witnessed_with_low = (fun _ -> True);
+  }
+
 
 open STLC
 
@@ -139,7 +128,7 @@ let rec _elab_typ (t:typ) : tt:Type & target_lang tt =
     (| (tt1 * tt2), target_lang_pair tt1 tt2 #c_tt1 #c_tt2 |)
   | TRef t ->
     let (| tt, c_tt |) = _elab_typ t in
-    (| lref tt, target_lang_ref tt #c_tt |)
+    (| ref tt, target_lang_ref tt #c_tt |)
 
 let elab_typ (t:typ) : Type =
   dfst (_elab_typ t)
@@ -150,72 +139,67 @@ let elab_typ_tgt (t:typ) : target_lang (elab_typ t)=
 
 
 (** ** Examples **) 
-let write' (#t:Type) {| c:target_lang t |} (r:lref t) (v:t) 
-: ST unit
+let write' (#t:Type) {| c:target_lang t |} (r:ref t) (v:t) 
+: IST unit
   (requires (fun h0 -> 
-    h0 `contains` r /\ 
-    label_of r h0 == Low /\ 
-
-    h0 `c.deep_contains` v /\
-    c.deeply_labeled_with_low v h0))
+    witnessed (is_low_pred r) /\
+    c.witnessed_with_low v))
   (ensures (fun h0 () h1 ->
     write_post r v h0 () h1 /\
     modifies_only_label Low h0 h1 /\
-    deeply_labeled_with_low r h1))
+    witnessed_with_low r))
 = let h0 = get () in
+  gst_recall (is_low_pred r);
+  recall r;
   r := v;
   let h1 = get () in
-  assume (deeply_labeled_with_low r h1);
+  assume (inv_low_points_to_low h1);
   ()
 
 
 val alloc' (#a:Type) {| c:target_lang a |} (init:a)
-: ST (lref a)
-  (requires (fun h0 ->
-    c.deeply_labeled_with_low init h0
-    ))
+: IST (ref a)
+  (requires (fun h0 -> 
+    c.witnessed_with_low init))
   (ensures (fun h0 r h1 -> 
     fresh r h0 h1 /\ 
     modifies Set.empty h0 h1 /\
     modifies_classification Set.empty h0 h1 /\
     sel h1 r == init /\ 
-    deeply_labeled_with_low r h1
-    ))
+    witnessed_with_low r))
 let alloc' #_ #c init = 
   let r = alloc init in
-  let r' = declassify_low r in
-  let h1 = get () in
-  assume (deeply_labeled_with_low r' h1);
-  r'
+  declassify r Low;
+  gst_witness (is_low_pred r);
+  r
 
 val ctx_update_ref_test : 
   elab_typ (TArr (TRef TNat) TUnit)
-let ctx_update_ref_test (y:lref int) =
+let ctx_update_ref_test (y:ref int) =
   write' y (!y + 5);
   ()
 
 val ctx_update_multiple_refs_test : 
   elab_typ (TArr (TRef (TRef TNat)) (TArr (TRef TNat) TUnit))
-let ctx_update_multiple_refs_test (x:lref (lref int)) (y:lref int) =
-  deep_recall x; (* Fstar forgets that x is contained and low **)
-  let ix : lref int = !x in
+let ctx_update_multiple_refs_test (x:ref (ref int)) (y:ref int) =
+  let ix : ref int = !x in
+  let h0 = get () in
+  eliminate forall (a:Type) (c:target_lang a) (r:ref a). witnessed (is_low_pred r) ==>
+    c.witnessed_with_low (sel h0 r) with (ref int) (solve) x;
   write' ix (!ix + 1);
-  deep_recall x; (* TODO: why is this one needed? *)
   write' x y;
   write' y (!y + 5);
   ()
 
 val ctx_HO_test1 : 
   elab_typ (TArr (TRef (TPair (TRef TNat) (TRef TNat))) (TArr TUnit TUnit))
-let ctx_HO_test1 (xs:lref ((lref int) * lref int)) =
+let ctx_HO_test1 (xs:ref ((ref int) * ref int)) =
   let (x', x'') = !xs in
+  let h0 = get () in
+  eliminate forall (a:Type) (c:target_lang a) (r:ref a). witnessed (is_low_pred r) ==>
+    c.witnessed_with_low (sel h0 r) with ((ref int) * (ref int)) (solve) xs;
   write' xs (x', x');  // xs := (x', x');
-  (fun () ->
-    deep_recall xs;
-    deep_recall x';
-    deep_recall x'';
-    write' xs (x', x'')
-  )
+  (fun () -> write' xs (x', x''))
   
 val ctx_identity :
   elab_typ (TArr (TRef TNat) (TRef TNat))
@@ -225,22 +209,19 @@ val ctx_HO_test2 :
   elab_typ (TArr (TArr TUnit (TRef TNat)) TUnit)
 let ctx_HO_test2 f =
   let h0 = get () in
-  let x:lref int = f () in
+  let x:ref int = f () in
   let h1 = get () in
-  // assume (lheap_rel h0 h1);
-  // assert (modifies_only_label Low h0 h1);
   write' x (!x + 1);
   let h2 = get () in
-  // assume (lheap_rel h1 h2);
-  // assert (modifies_only_label Low h1 h2);
-  // assert (objects_deeply_labeled h2);
   assert (modifies_only_label Low h0 h2);
   ()
 
 val ctx_swap_ref_test :
   elab_typ (TArr (TRef (TRef TNat)) (TArr (TRef (TRef TNat)) TUnit))
-let ctx_swap_ref_test (x y: lref (lref int)) =
-  deep_recall x;
+let ctx_swap_ref_test (x y: ref (ref int)) =
+  let h0 = get () in
+  eliminate forall (a:Type) (c:target_lang a) (r:ref a). witnessed (is_low_pred r) ==>
+    c.witnessed_with_low (sel h0 r) with (ref int) (solve) x;
   let z = !x in
   let t = !y in
   write' x t;
@@ -263,10 +244,8 @@ let ctx_HO_test3 f =
 val ctx_returns_callback_test :
   elab_typ (TArr TUnit (TArr TUnit TUnit))
 let ctx_returns_callback_test () =
-  let x: lref int = alloc' 13 in
+  let x: ref int = alloc' 13 in
   let cb : elab_typ (TArr TUnit TUnit) = (fun() ->
-    deep_recall x;
-    let h0 = get () in
     write' x (!x % 5)
   ) in
   cb
@@ -274,8 +253,8 @@ let ctx_returns_callback_test () =
 val ctx_HO_test4 :
   elab_typ (TArr (TArr TUnit (TRef TNat)) TUnit)
 let ctx_HO_test4 f =
-  let x:lref int = f () in
-  let y:lref (lref int) = alloc' x in
+  let x:ref int = f () in
+  let y:ref (ref int) = alloc' x in
   ()
 
 val progr_sep_test: 
@@ -283,92 +262,95 @@ val progr_sep_test:
   ctx:(elab_typ (TArr TUnit TUnit)) ->
   ST unit
     (requires (fun h0 -> 
-      h0 `contains` rp /\
+      inv_low_points_to_low h0 /\
       label_of rp h0 == High))
     (ensures (fun h0 _ h1 ->
       sel h0 rp == sel h1 rp)) // the content of rp should stay the same before/ after calling the context
          
 let progr_sep_test #rp f = (** If this test fails, it means that the spec of f does not give [automatically] separation  **)
+  recall rp;
   f ()
 
 val progr_sep_test_alloc:
   #rp: ref int -> 
   ctx:(elab_typ (TArr (TRef TNat) TUnit)) ->
-  ST unit
+  IST unit
     (requires (fun h0 -> 
-      h0 `contains` rp /\
       label_of rp h0 == High))
     (ensures (fun h0 _ h1 -> True))
 let progr_sep_test_alloc #rp f =
   f (declassify_low rp)
 
 val progr_sep_test_nested:
-  #rp: ref (ref int) -> 
+  rp: ref (ref int) -> 
   ctx:(elab_typ (TArr (TRef (TRef TNat)) TUnit)) ->
-  ST unit
+  IST unit
     (requires (fun h0 -> 
-      h0 `contains` rp /\
       label_of rp h0 == High))
     (ensures (fun h0 _ h1 -> True))
-let progr_sep_test_nested #rp f =
+let progr_sep_test_nested rp f =
   declassify rp Low; gst_witness (is_low_pred rp);
   let p = !rp in
   declassify p Low; gst_witness (is_low_pred p);
-  let r = alloc' (!rp) in (* <-- needed a copy here! *) 
-  f r
+  // let r = alloc' (!rp) in (* <-- needed a copy here! *) 
+  f rp
 
 val progr_secret_unchanged_test: 
-  #rp: ref int -> 
-  #rs: lref (lref int) ->
+  rp: ref int -> 
+  rs: ref (ref int) ->
   ctx:(elab_typ (TArr TUnit TUnit)) ->
-  ST unit 
+  IST unit 
     (requires (fun h0 -> 
-      h0 `contains` rp /\
-      h0 `deep_contains` rs /\
       label_of rp h0 == High /\
-      deeply_labeled_with_low rs h0))
-    (ensures (fun h0 _ h1 -> 
+      witnessed (is_low_pred rs)))
+    (ensures (fun h0 _ h1 ->
       sel h0 rp == sel h1 rp))
          
-let progr_secret_unchanged_test #_ #rs ctx = 
+let progr_secret_unchanged_test rp rs ctx = 
+  recall rp; (* This has to be very precisely here! *)
   let secret: ref int = alloc 0 in
+  let h0 = get () in
+  assume (inv_low_points_to_low h0);
   ctx ();
   let v = !secret in
   assert (v == 0);
   ()
 
 val progr_passing_callback_test: 
-  #rp: ref int -> 
-  #rs: lref (lref int) ->
+  rp: ref int -> 
+  rs: ref (ref int) ->
   ctx:(elab_typ (TArr (TArr TUnit TUnit) TUnit)) ->
-  ST unit 
-    (requires (fun h0 -> 
-      h0 `contains` rp /\
-      h0 `deep_contains` rs /\
+  IST unit 
+    (requires (fun h0 ->
       label_of rp h0 == High /\
-      deeply_labeled_with_low rs h0))
+      witnessed (is_low_pred rs)))
     (ensures (fun h0 _ h1 -> sel h0 rp == sel h1 rp)) // the content of rp should stay the same before/ after calling the context
 
 // TODO: the callback of the program should be able to modify rp
-let progr_passing_callback_test #_ #rs f =
-  let secret: lref int = alloc' 0 in
-  let cb: elab_typ (TArr TUnit TUnit) = (fun () -> deep_recall secret; write' secret (!secret + 1)) in
+let progr_passing_callback_test rp rs f =
+  recall rp;
+  let secret: ref int = alloc 0 in
+  declassify secret Low; gst_witness (is_low_pred secret);
+  let h0 = get () in
+  assume (inv_low_points_to_low h0);
+
+  let cb: elab_typ (TArr TUnit TUnit) = (fun () -> 
+    gst_recall (is_low_pred secret);
+    write' secret (!secret + 1)) in
   f cb;
   ()
 
 val progr_getting_callback_test: 
-  #rp: ref int -> 
-  #rs: lref (lref int) ->
+  rp: ref int -> 
+  rs: ref (ref int) ->
   ctx:(elab_typ (TArr TUnit (TArr TUnit TUnit))) ->
-  ST unit 
-    (requires (fun h0 -> 
-      h0 `contains` rp /\
-      h0 `deep_contains` rs /\
+  IST unit 
+    (requires (fun h0 ->
       label_of rp h0 == High /\
-      deeply_labeled_with_low rs h0))
+      witnessed (is_low_pred rs)))
     (ensures (fun h0 _ h1 -> sel h0 rp == sel h1 rp))
-
-let progr_getting_callback_test #_ #rs f =
+let progr_getting_callback_test rp rs f =
+  recall rp;
   let h0 = get () in
   let cb = f () in
   cb ();
@@ -389,11 +371,11 @@ let elab_apply_arrow t1 t2 f x = f x
 let cast_TArr #t1 #t2 (f : elab_typ (TArr t1 t2)) (t:typ) (#_:squash (t == TArr t1 t2)) : elab_typ t = f
 
 type vcontext (g:context) = 
-  vx:var{Some? (g vx)} -> elab_typ (Some?.v (g vx))
+  vx:var{Some? (g vx)} -> x:(elab_typ (Some?.v (g vx))){(elab_typ_tgt (Some?.v (g vx))).witnessed_with_low x}
 
 let vempty : vcontext empty = fun _ -> assert false
 
-let vextend #t (x:elab_typ t) (#g:context) (ve:vcontext g) : vcontext (extend t g) =
+let vextend #t (x:(elab_typ t){(elab_typ_tgt t).witnessed_with_low x}) (#g:context) (ve:vcontext g) : vcontext (extend t g) =
   fun y -> if y = 0 then x else ve (y-1)
 
 #push-options "--split_queries always"
@@ -403,7 +385,7 @@ let rec elab_exp
   (#t:typ)
   (tyj:typing g e t)
   (ve:vcontext g)
-  : ST (elab_typ t) 
+  : IST (elab_typ t) 
      (requires (pre_tgt_arrow () #target_lang_unit))
      (ensures (post_tgt_arrow () #_ #(fun _ -> elab_typ t) #(fun _ -> elab_typ_tgt t))) =
   let h0 = get () in
@@ -415,16 +397,15 @@ let rec elab_exp
 
   | TyAllocRef #_ #_ #t tyj_e -> begin
     let v : elab_typ t = elab_exp tyj_e ve in
-    let r : lref (elab_typ t) = alloc' #_ #(elab_typ_tgt t) v in
-    (elab_typ_tgt (TRef t)).deep_recall r;
+    let r : ref (elab_typ t) = alloc' #_ #(elab_typ_tgt t) v in
     r
   end
   | TyReadRef #_ #_ #t tyj_e -> begin
-    let r : lref (elab_typ t) = elab_exp tyj_e ve in
+    let r : ref (elab_typ t) = elab_exp tyj_e ve in
     !r
   end
   | TyWriteRef #_ #_ #_ #t tyj_ref tyj_v -> begin
-      let r : lref (elab_typ t) = elab_exp tyj_ref ve in
+      let r : ref (elab_typ t) = elab_exp tyj_ref ve in
       let v : elab_typ t = elab_exp tyj_v ve in
       write' #_ #(elab_typ_tgt t) r v
   end
@@ -439,13 +420,11 @@ let rec elab_exp
   | TyVar vx -> 
     let Some tx = g vx in
     let x : elab_typ tx = ve vx in
-    (elab_typ_tgt tx).deep_recall x;
     x
   | TyApp #_ #_ #_ #tx #tres tyj_f tyj_x ->
     assert ((elab_typ t) == (elab_typ tres));
     let x : elab_typ tx = elab_exp tyj_x ve in
     let f : elab_typ (TArr tx tres) = elab_exp tyj_f ve in
-    (elab_typ_tgt tx).deep_recall x;
     elab_apply_arrow tx tres f x
 
   | TyInl #_ #_ #t1 #t2 tyj_1 ->
@@ -459,11 +438,9 @@ let rec elab_exp
     match vc with 
     | Inl x -> 
       let f : elab_typ (TArr tl tres) = elab_exp tyj_l ve in
-      (elab_typ_tgt tl).deep_recall x;
       elab_apply_arrow tl tres f x
     | Inr y ->
       let f : elab_typ (TArr tr tres) = elab_exp tyj_r ve in
-      (elab_typ_tgt tr).deep_recall y;
       elab_apply_arrow tr tres f y
   end
 
@@ -476,6 +453,5 @@ let rec elab_exp
   | TyPair #_ #_ #_ #tf #ts tyj_f tyj_s->
     let vf : elab_typ tf = elab_exp tyj_f ve in
     let vs : elab_typ ts = elab_exp tyj_s ve in
-    (elab_typ_tgt tf).deep_recall vf;
     (vf, vs)
-  #pop-options
+#pop-options
